src/QUIC.Secret.Seq.fsti
@@ -1,0 +1,109 @@
+module QUIC.Secret.Seq
+include FStar.Seq
+
+module Secret = QUIC.Secret.Int
+module U8 = FStar.UInt8
+module Ghost = FStar.Ghost
+
+noextract
+val seq_hide
+  (#t: Secret.inttype { Secret.unsigned t })
+  (#sec: Secret.secrecy_level)
+  (x: seq (Secret.uint_t t sec))
+: Tot (seq (Secret.uint_t t Secret.SEC))
+
+val seq_hide_length
+  (#t: Secret.inttype { Secret.unsigned t })
+  (#sec: Secret.secrecy_level)
+  (x: seq (Secret.uint_t t sec))
+: Lemma
+  (length (seq_hide x) == length x)
+  [SMTPat (length (seq_hide x))]
+
+val seq_hide_index
+  (#t: Secret.inttype { Secret.unsigned t })
+  (#sec: Secret.secrecy_level)
+  (x: seq (Secret.uint_t t sec))
+  (i: nat)
+: Lemma
+  (requires (i < length x))
+  (ensures (
+    Secret.v (index (seq_hide x) i) == Secret.v (index x i)
+  ))
+  [SMTPat (index (seq_hide x) i)]
+
+let seq_hide_sec
+  (#t: Secret.inttype { Secret.unsigned t })
+  (x: seq (Secret.uint_t t Secret.SEC))
+: Lemma
+  (seq_hide x `equal` x)
+= ()
+
+val seq_reveal
+  (#t: Secret.inttype { Secret.unsigned t })
+  (#sec: Secret.secrecy_level)
+  (x: seq (Secret.uint_t t sec))
+: GTot (seq (Secret.uint_t t Secret.PUB))
+
+val seq_reveal_length
+  (#t: Secret.inttype { Secret.unsigned t })
+  (#sec: Secret.secrecy_level)
+  (x: seq (Secret.uint_t t sec))
+: Lemma
+  (length (seq_reveal x) == length x)
+  [SMTPat (length (seq_reveal x))]
+
+val seq_reveal_index
+  (#t: Secret.inttype { Secret.unsigned t })
+  (#sec: Secret.secrecy_level)
+  (x: seq (Secret.uint_t t sec))
+  (i: nat)
+: Lemma
+  (requires (i < length x))
+  (ensures (
+    Secret.v (index (seq_reveal x) i) == Secret.v (index x i)
+  ))
+  [SMTPat (index (seq_reveal x) i)]
+
+let seq_reveal_pub
+  (#t: Secret.inttype { Secret.unsigned t })
+  (x: seq (Secret.uint_t t Secret.PUB))
+: Lemma
+  (seq_reveal x `equal` x)
+= ()
+
+let seq_reveal_hide
+  (#t: Secret.inttype { Secret.unsigned t })
+  (x: seq (Secret.uint_t t Secret.PUB))
+: Lemma
+  (seq_reveal (seq_hide x) `equal` x)
+= ()
+
+let seq_hide_reveal
+  (#t: Secret.inttype { Secret.unsigned t })
+  (x: seq (Secret.uint_t t Secret.SEC))
+: Lemma
+  (seq_hide (seq_reveal x) `equal` x)
+= ()
+
+let seq_reveal_inj
+  (#t: Secret.inttype { Secret.unsigned t })
+  (#sec: Secret.secrecy_level)
+  (x1 x2: seq (Secret.uint_t t sec))
+: Lemma
+  (requires (seq_reveal x1 `equal` seq_reveal x2))
+  (ensures (x1 `equal` x2))
+= match sec with
+  | Secret.PUB -> seq_reveal_pub #t x1; seq_reveal_pub #t x2
+  | Secret.SEC -> seq_hide_reveal #t x1; seq_hide_reveal #t x2
+
+let seq_hide_inj
+  (#t: Secret.inttype { Secret.unsigned t })
+  (#sec: Secret.secrecy_level)
+  (x1 x2: seq (Secret.uint_t t sec))
+: Lemma
+  (requires (seq_hide x1 `equal` seq_hide x2))
+  (ensures (x1 `equal` x2))
+= match sec with
+  | Secret.SEC -> seq_hide_sec #t x1; seq_hide_sec #t x2
+  | Secret.PUB -> seq_reveal_hide #t x1; seq_reveal_hide #t x2
